dsn/Lang/Dynamic/NStep.lean
@@ -105,6 +105,12 @@ mutual
 end
 
 
+theorem NStep.iso_choice :
+  NStep (Expr.iso label body) e →
+  ∃ body_choice , e = (Expr.iso label body_choice) ∧  NStep body body_choice
+:= by
+  sorry
+
 theorem NStep.project : NStep (Expr.project (Expr.record [(l, e)]) l) e := by
   unfold Expr.project
   have h0 : Expr.pattern_match
